theories/rules/rules_EInit.v
@@ -33,14 +33,18 @@ Section cap_lang_rules.
       EInit_fail lregs lmem ot.
 
   Inductive EInit_spec (lregs lregs' : LReg) (lmem lmem' : LMem) (n n' : nat) (tidx : TIndex) (eid : EIdentity) (ot : OType) (rs : RegName) : cap_lang.val → Prop :=
-    | EInit_success_no_revoke code_b code_e code_a code_v data_b data_e data_a data_v :
+    | EInit_success_no_revoke code_b code_e code_a code_v data_b data_e data_a data_v vmap :
       incrementLPC lregs = Some lregs' →
       n + 1 = n' →
+      eid = hash_lmemory_region lmem code_b code_e code_v →
       (ot + 2)%ot = Some (ot ^+ 2)%ot →
       lregs !! rs = Some (LCap RX code_b code_e code_a code_v) →
       lmem !! (code_b, code_v) = Some (LCap RW data_b data_e data_a data_v) →
-      is_valid_updated_lmemory lmem (finz.seq_between code_b code_e) code_v lmem' -> (* support revocation *)
-      is_valid_updated_lmemory lmem (finz.seq_between data_b data_e) data_v lmem' -> (* support revocation *)
+      is_valid_updated_lmemory lmem (finz.seq_between code_b code_e) code_v lmem' → (* support revocation *)
+      is_valid_updated_lmemory lmem (finz.seq_between data_b data_e) data_v lmem' → (* support revocation *)
+      unique_in_registersL lregs rs (LCap RX code_b code_e code_a code_v) →
+      unique_in_memoryL lmem vmap code_b → (* @TODO: I'm missing something for sure... *)
+      incrementLPC (<[ rs := LInt eid]> lregs) = Some lregs' →
       EInit_spec lregs lregs' lmem lmem' n n' tidx eid ot rs NextIV
     | EInit_failure :
       n = n' →
@@ -48,8 +52,7 @@ Section cap_lang_rules.
       EInit_spec lregs lregs' lmem lmem' n n' tidx eid ot rs FailedV.
 
   (* TODO: Failure lmem does not contain none at code_b etc *)
-  (* TODO: how to determine tidx and eid in the spec? *)
-  (* TODO: hash? *)
+  (* TODO: how to determine tidx *)
   (* TODO @Denis *)
   Lemma wp_einit E pc_p pc_b pc_e pc_a pc_v pc_a' lw
     lregs lmem tidx eid rs n :
@@ -71,8 +74,8 @@ Section cap_lang_rules.
         [∗ map] la↦lw ∈ lmem', la ↦ₐ lw ∗
         [∗ map] k↦y ∈ lregs', k ↦ᵣ y ∗
         EC⤇ n' ∗ (* need to give back the fragment of EC *)
-        (* gain a non-duplicable token that asserts ownership over the enclave at etable index `tidx` *)
-        if decide (retv = NextIV) then
+        if decide (retv = NextIV) then (* if EInit was successful *)
+          (* gain a non-duplicable token that asserts ownership over the enclave at etable index `tidx` *)
           enclave_cur tidx eid
           (* @TODO Denis/June: seal predicates needed? *)
         else emp }}}.
